partial/Lambda.v
@@ -5,7 +5,9 @@ Require Import ListIndex.
 Require Import Tactics.
 Require Import Coq.Program.Equality.
 Module Lambda (mem : Memory).
-Import mem.
+Module Mem := MemoryTheory mem.
+Import Mem.
+
 
 (** * Syntax *)
 
@@ -90,13 +92,13 @@ Inductive Elem : Set :=
 | CLO : Code -> Env' -> Elem
 .
 
-Inductive Conf : Set := 
-| conf : Code -> Value' -> Env' -> Conf.
+Inductive Conf : Type := 
+| conf : Code -> Value' -> Env' -> Mem Elem -> Conf.
 
-Notation "⟨ c , a , e , s ⟩" := (conf c a e, s).
+Notation "⟨ c , a , e , s ⟩" := (conf c a e s).
 
 Reserved Notation "x ==> y" (at level 80, no associativity).
-Inductive VM : Conf * Mem Elem -> Conf * Mem Elem -> Prop :=
+Inductive VM : Conf -> Conf -> Prop :=
  | vm_push n c s a e :  ⟨LOAD n c, a, e, s⟩ ==> ⟨c, Num' n, e, s⟩ 
  | vm_add c m n r s e : s[r] = VAL (Num' m) -> ⟨ADD r c, Num' n, e, s⟩ 
                                                  ==> ⟨c, Num'(m + n), e, s⟩
@@ -120,19 +122,25 @@ Fixpoint conv (v : Value) : Value' :=
 
 Definition convE : Env -> Env' := map conv.
 
+
+Inductive cle : Conf -> Conf -> Prop :=
+ | cle_mem  c a e s s' : s ≤ s' -> cle ⟨ c , a , e , s ⟩ ⟨ c , a , e , s' ⟩.
+
+Hint Constructors cle.
+
+
 (** * Calculation *)
 
 (** Boilerplate to import calculation tactics *)
-
-Module Mon := Monotonicity mem.
-Import Mon.
-
-Module VM <: (Machine mem).
+Module VM <: Machine.
 Definition Conf := Conf.
+Definition Pre := cle.
 Definition Rel := VM.
-Definition MemElem := Elem.
-Lemma monotone : monotonicity VM.
+Definition MemElem := nat.
+Lemma monotone : monotonicity cle VM.
 prove_monotonicity. Qed.
+Lemma preorder : is_preorder cle.
+prove_preorder. Qed.
 End VM.
 Module VMCalc := Calculation mem VM.
 Import VMCalc.
