partial/LambdaStack.v
@@ -5,7 +5,9 @@ Require Import ListIndex.
 Require Import Tactics.
 Require Import Coq.Program.Equality.
 Module Lambda (mem : Memory).
-Import mem.
+Module Mem := MemoryTheory mem.
+Import Mem.
+
 
 (** * Syntax *)
 
@@ -61,7 +63,7 @@ Inductive Code : Set :=
 | ADD : adr -> Code -> Code
 | STORE : adr -> Code -> Code
 | LOOKUP : nat -> Code -> Code
-| RET : adr -> Code
+| RET : Code
 | APP : adr -> Code -> Code
 | ABS : Code -> Code -> Code
 | POP : Code -> Code
@@ -73,7 +75,7 @@ Fixpoint comp' (e : Expr) (r : adr) (c : Code) : Code :=
     | Add x y => comp' x r (STORE r (comp' y (next r) (ADD r c)))
     | Var i => LOOKUP i c
     | App x y => comp' x r (STORE r (comp' y (next r) (APP r (POP c))))
-    | Abs x => ABS (comp' x (next adr0) (RET adr0)) c
+    | Abs x => ABS (comp' x (next adr0) RET) c
   end.
 
 Definition comp (e : Expr) : Code := comp' e adr0 HALT.
@@ -96,12 +98,12 @@ Notation empty := (empty_mem Elem).
 Definition Stack : Type := list (Mem Elem).
 
 Inductive Conf : Type := 
-| conf : Code -> Value' -> Env' -> Stack -> Conf.
+| conf : Code -> Value' -> Env' -> Stack -> Mem Elem -> Conf.
 
-Notation "⟨ c , a , e , k , s ⟩" := (conf c a e k, s).
+Notation "⟨ c , a , e , k , s ⟩" := (conf c a e k s).
 
 Reserved Notation "x ==> y" (at level 80, no associativity).
-Inductive VM : Conf * Mem Elem -> Conf * Mem Elem -> Prop :=
+Inductive VM : Conf -> Conf -> Prop :=
  | vm_push n c s a e k :  ⟨LOAD n c, a, e, k, s⟩ ==> ⟨c, Num' n, e, k, s⟩
  | vm_pop c s s' a e k :  ⟨POP c, a, e, s' :: k, s⟩ ==> ⟨c, a, e, k, s'⟩
  | vm_add c m n r s e k : s[r] = VAL (Num' m) -> ⟨ADD r c, Num' n, e, k, s⟩
@@ -109,10 +111,10 @@ Inductive VM : Conf * Mem Elem -> Conf * Mem Elem -> Prop :=
  | vm_store c v r s e k : ⟨STORE r c, v, e, k, s⟩
                         ==> ⟨c, v, e, k, s[r:=VAL v]⟩
  | vm_lookup e i c v a s k : nth e i = Some v -> ⟨LOOKUP i c, a, e, k, s⟩ ==> ⟨c, v, e, k, s⟩
- | vm_env a r c e e' s k : s[r] = CLO c e -> ⟨RET r, a, e', k, s⟩ ==> ⟨c, a, e, k, s⟩
+ | vm_env a c e e' s k : s[adr0] = CLO c e -> ⟨RET, a, e', k, s⟩ ==> ⟨c, a, e, k, s⟩
  | vm_app c c' e e' v r s k :
      s[r]=VAL (Clo' c' e') ->
-     ⟨APP r c, v, e, k,s⟩ ==> ⟨c', Num' 0, v :: e', truncate r s :: k, empty[adr0:=CLO c e]⟩
+     ⟨APP r c, v, e, k,s⟩ ==> ⟨c', Num' 0, v :: e', s :: k, empty[adr0:=CLO c e]⟩
  | vm_abs a c c' s e k : ⟨ABS c' c, a, e, k, s⟩ ==> ⟨c, Clo' c' e, e, k, s⟩
 where "x ==> y" := (VM x y).
 
@@ -121,41 +123,86 @@ where "x ==> y" := (VM x y).
 Fixpoint conv (v : Value) : Value' :=
   match v with
     | Num n => Num' n
-    | Clo x e => Clo' (comp' x (next adr0) (RET adr0)) (map conv e)
+    | Clo x e => Clo' (comp' x (next adr0) RET) (map conv e)
   end.
 
 Definition convE : Env -> Env' := map conv.
+
+Inductive stackle : Stack -> Stack -> Prop :=
+| stackle_empty : stackle nil nil
+| stackle_cons s s' k k' : s ≤ s' -> stackle k k' -> stackle (s :: k) (s' :: k').
+
+Hint Constructors stackle : memory.
+
+Lemma stackle_refl k : stackle k k.
+Proof.
+  induction k; constructor; auto with memory.
+Qed.
+
+Lemma stackle_trans k1 k2 k3 : stackle k1 k2 -> stackle k2 k3 -> stackle k1 k3.
+Proof.
+  intros L1. generalize k3. induction L1; intros k3' L2. assumption. inversion L2. subst. constructor;
+  eauto with memory.
+Qed.
+
+Hint Resolve stackle_refl stackle_trans.
+
+Inductive cle : Conf -> Conf -> Prop :=
+ | cle_mem  c a e k k' s s' : stackle k k' -> s ≤ s' -> cle ⟨ c , a , e , k, s ⟩ ⟨ c , a , e , k', s' ⟩.
+
+Hint Constructors cle.
+
+Lemma rel_eq {T} {R : T -> T -> Prop} x y y' : R x y' -> y = y' -> R x y.
+Proof. intros. subst. auto.
+Qed .
+Lemma rel_eq' {T} {R : T -> T -> Prop} x x' y : R x' y -> x = x' -> R x y.
+Proof. intros. subst. auto.
+Qed .
+
+Ltac apply_eq t := eapply rel_eq; [apply t | repeat rewrite set_set; auto].
+
 
 (** * Calculation *)
 
 (** Boilerplate to import calculation tactics *)
 
-Module Mon := Monotonicity mem.
-Import Mon.
-
-
-
-Lemma rel_eq {T} {R : T -> T -> Prop} x y y' : R x y' -> y = y' -> R x y.
-Proof. intros. subst. auto.
-Qed .
-Ltac apply_eq t := eapply rel_eq; [apply t | repeat rewrite set_set; auto].
-
-Module VM <: (Machine mem).
+Module VM <: Machine.
 Definition Conf := Conf.
+Definition Pre := cle.
 Definition Rel := VM.
-Definition MemElem := Elem.
-Lemma monotone : monotonicity VM.
-  do 5 intro; intros Hle Step;
-  dependent destruction Step;
-  try (eexists; (split; [econstructor| idtac]); eauto using memle_get, set_monotone).
-  eexists (empty [adr0 := CLO c e]). split. apply_eq vm_app. eauto using memle_get, set_monotone. 
+Definition MemElem := nat.
+Lemma monotone : monotonicity cle VM.
+  prove_monotonicity1;
+    try (match goal with [H : stackle (_ :: _) _ |- _] => inversion H end)
+    ; prove_monotonicity2.
+Qed.
+Lemma preorder : is_preorder cle.
+prove_preorder. Qed.
+End VM.
 
-  apply Hle in H.
+
+
+(* Lemma rel_eq {T} {R : T -> T -> Prop} x y y' : R x y' -> y = y' -> R x y. *)
+(* Proof. intros. subst. auto. *)
+(* Qed . *)
+(* Ltac apply_eq t := eapply rel_eq; [apply t | repeat rewrite set_set; auto]. *)
+
+(* Module VM <: (Machine mem). *)
+(* Definition Conf := Conf. *)
+(* Definition Rel := VM. *)
+(* Definition MemElem := Elem. *)
+(* Lemma monotone : monotonicity VM. *)
+(*   do 5 intro; intros Hle Step; *)
+(*   dependent destruction Step; *)
+(*   try (eexists; (split; [econstructor| idtac]); eauto using memle_get, set_monotone). *)
+(*   eexists (empty [adr0 := CLO c e]). split. apply_eq vm_app. eauto using memle_get, set_monotone.  *)
+
+(*   apply Hle in H. *)
 
   
-  Admitted.
-(* prove_monotonicity. Qed. *)
-End VM.
+(*   Admitted. *)
+
+
 Module VMCalc := Calculation mem VM.
 Import VMCalc.
 
@@ -192,7 +239,7 @@ Proof.
 
   begin
     ⟨c, Num' (m + n), convE e, k, s⟩.
-  ≤ { auto }
+  ≤ {auto}
     ⟨c, Num' (m + n), convE e, k, s[r:=VAL (Num' m)]⟩ .
   <== { apply vm_add }
     ⟨ADD r c, Num' n, convE e, k, s[r:=VAL (Num' m)]⟩ .
@@ -215,9 +262,9 @@ Proof.
 (** - [Abs x ⇓[e] Clo x e] *)
 
   begin
-    ⟨c, Clo' (comp' x (next adr0) (RET adr0)) (convE e), convE e, k, s ⟩.
+    ⟨c, Clo' (comp' x (next adr0) RET) (convE e), convE e, k, s ⟩.
   <== { apply vm_abs }
-    ⟨ABS (comp' x (next adr0) (RET adr0)) c, a, convE e, k, s ⟩.
+    ⟨ABS (comp' x (next adr0) RET) c, a, convE e, k, s ⟩.
   [].
 
 (** - [App x y ⇓[e] x''] *)
@@ -227,17 +274,19 @@ Proof.
   <== { apply vm_pop }
     ⟨POP c, conv x'', convE e, s :: k, empty[adr0:=CLO (POP c) (convE e)] ⟩.
   <== { apply vm_env }
-    ⟨RET adr0, conv x'', convE (y' :: e'), s :: k, empty[adr0:=CLO (POP c) (convE e)]⟩.
+    ⟨RET, conv x'', convE (y' :: e'), s :: k, empty[adr0:=CLO (POP c) (convE e)]⟩.
   <|= {apply  IHE3}
-      ⟨comp' x' (next adr0) (RET adr0), Num' 0, convE (y' :: e'), s :: k, empty[adr0:=CLO (POP c) (convE e)]⟩.
+      ⟨comp' x' (next adr0) RET, Num' 0, convE (y' :: e'), s :: k, empty[adr0:=CLO (POP c) (convE e)]⟩.
   = {auto}
-      ⟨comp' x' (next adr0) (RET adr0), Num' 0, conv y' :: convE e', s::k, empty[adr0:=CLO (POP c) (convE e)]⟩.
+      ⟨comp' x' (next adr0) RET, Num' 0, conv y' :: convE e', s::k, empty[adr0:=CLO (POP c) (convE e)]⟩.
+  ≤ {auto with memory}
+      ⟨comp' x' (next adr0) RET, Num' 0, conv y' :: convE e', s[r:=VAL (Clo' (comp' x' (next adr0) RET) (convE e'))]::k, empty[adr0:=CLO (POP c) (convE e)]⟩.
   <== {apply_eq vm_app}
-      ⟨APP r (POP c), conv y', convE e, k, s[r:=VAL (Clo' (comp' x' (next adr0) (RET adr0)) (convE e'))]⟩.
+      ⟨APP r (POP c), conv y', convE e, k, s[r:=VAL (Clo' (comp' x' (next adr0) RET) (convE e'))]⟩.
   <|= {apply IHE2}
-      ⟨comp' y (next r) (APP r (POP c)), (Clo' (comp' x' (next adr0) (RET adr0)) (convE e')), convE e, k, s[r:=VAL (Clo' (comp' x' (next adr0) (RET adr0)) (convE e'))]⟩.
+      ⟨comp' y (next r) (APP r (POP c)), (Clo' (comp' x' (next adr0) RET) (convE e')), convE e, k, s[r:=VAL (Clo' (comp' x' (next adr0) RET) (convE e'))]⟩.
   <== { apply vm_store }
-    ⟨STORE r (comp' y (next r) (APP r (POP c))), (Clo' (comp' x' (next adr0) (RET adr0)) (convE e')), convE e, k, s⟩.
+    ⟨STORE r (comp' y (next r) (APP r (POP c))), (Clo' (comp' x' (next adr0) RET) (convE e')), convE e, k, s⟩.
   = {auto}
     ⟨STORE r (comp' y (next r) (APP r (POP c))), conv (Clo x' e'), convE e, k, s ⟩.
   <|= { apply IHE1 }
@@ -254,14 +303,14 @@ Qed.
 
 Definition terminates (p : Expr) : Prop := exists r, p ⇓[nil] r.
 
-Theorem sound p a s C : freeFrom adr0 s -> terminates p -> ⟨comp p, a, nil, s⟩ =>>! C -> 
-                          exists v s', C = ⟨HALT , conv v, nil, s'⟩ /\ p ⇓[nil] v.
+Theorem sound p a s C : freeFrom adr0 s -> terminates p -> ⟨comp p, a, nil, nil, s⟩ =>>! C -> 
+                          exists v s', C = ⟨HALT , conv v, nil, nil, s'⟩ /\ p ⇓[nil] v.
 Proof.
   unfold terminates. intros F T M. destruct T as [v T].
-  pose (spec p v nil adr0 HALT a s F T) as H'.
+  pose (spec p v nil adr0 HALT a s nil F T) as H'.
   unfold Reach in *. repeat autodestruct.
   pose (determ_trc determ_vm) as D.
-  unfold determ in D. inversion H0. subst. exists v. eexists. split. eapply D. apply M. split.
+  unfold determ in D. inversion H0.  inversion H7.  subst. exists v. eexists. split. eapply D. apply M. split.
   unfold comp.
   simpl in *. apply H. intro Contra. destruct Contra.
   inversion H1. assumption.
